a dependently-typed version of to_action using Equations

noc/setup.v
@@ -6,34 +6,29 @@ From Coq Require Import Arith Lia Program.
 From Equations Require Import Equations.
 Require Import Coq.Vectors.Fin.
 
-Module Type Config.
-  Parameter nocsize: nat.
-  Axiom nocprop: 1<nocsize.
-End Config.
 
 Module Setup
-  (a : Config)
   (b : Typesize).
 
   Module c := Types b.
-  Import a c.
+  Import c.
 
   (** Router state
 
       Every router owns an internal state register.
-      For the pipeline every router owns the upstream transfer.
+      For the pipeline every router owns the downstream transfer.
    *)
   Inductive router_reg_t : Type :=
   | state
-  | upstream
+  | downstream
   .
 
   (** The pipeline
 
       The pipeline is essentially a list of routers.
    *)
-  Inductive reg_t : Type :=
-  | router : Fin.t nocsize -> router_reg_t -> reg_t
+  Inductive reg_t : nat -> Type :=
+  | router : forall x_dim, Fin.t (S x_dim) -> router_reg_t -> reg_t (S x_dim)
   .
 
   (** The router interface
@@ -50,8 +45,8 @@ Module Setup
 
       Every router has an interface.
    *)
-  Inductive ext_fn_t : Type :=
-  | ext_fun : Fin.t nocsize -> ext_com_t -> ext_fn_t
+  Inductive ext_fn_t : nat -> Type :=
+  | ext_fun : forall x_dim, Fin.t (S x_dim) -> ext_com_t -> ext_fn_t (S x_dim)
   .
 
   (** The Rules
@@ -61,386 +56,132 @@ Module Setup
       Hence, the schedule is simple: all routers run in parallel.
    *)
 
-  Inductive rule_name_t : Type :=
-  | rule : Fin.t nocsize -> rule_name_t.
+  Inductive rule_name_t : nat -> Type :=
+  | rule : forall x_dim, Fin.t (S x_dim) -> rule_name_t (S x_dim).
 
 End Setup.
 
 Module Actions
-  (a : Config)
+  (* (a : Config) *)
   (b : Typesize).
 
-  Module s := Setup a b.
-  Import s s.c.
+  Module s := Setup b.
   Module Routerfns:= Router b.
-  Import Routerfns.
+  Import s s.c Routerfns.
 
-Equations to_action {n:nat} {H1:n=nocsize} (rl : rule_name_t nocsize) :
-  uaction (reg_t regno) (ext_fn_t interfacesize) :=
+  Equations absurd_fin {T} (x:Fin.t 0) : T := .
 
-  @to_action O pf _rl := ! ;
-  @to_action 1 pf _rl := ! ;
-  @to_action (S noc_size') _pf (rule_ noc_size' idx) with idx :=
-    @to_action (S noc_size') _pf (rule noc_size' idx) (F1 0) :=
+  Derive NoConfusion for nat.
+  Derive NoConfusion for Fin.t.
+  Derive Signature for le.
+
+  (* Equations cannot recurse on [Prop]. *)
+  Fail Derive NoConfusion for le.
+
+  (* Set Equations Debug. *)
+
+  Equations widen_fin {n n'} (H: n<=n') (x : Fin.t n) : Fin.t n' :=
+    widen_fin (n:=0)   (n':=0)   _H          x := x;
+    widen_fin (n:=S a) (n':=S a) (le_n a)    x := x;
+    widen_fin (n:=0)   (n':=S a) _H  x := absurd_fin x; (* absurd *)
+    widen_fin (n:=S a) (n':=0)   H           x := _; (* absurd *)
+    widen_fin (n:=S a) (n':=S b) (le_S b H1) x with widen_fin H1 x => {
+        widen_fin (n:=S a) (n':=S b) (le_S b H2) _x y := FS y
+     }.
+  Next Obligation. lia.
+  Fail Qed.
+  (* Use [Set Equations Debug] to see more.
+     The problem is that Equations cannot recurse into [Prop] because
+     then the function become undefinable/extractable.
+   *)
+  Abort.
+
+
+  (* We recover from this situation by redefining [le] in [Type]. *)
+  Reserved Notation "a <<= b" (at level 99).
+  Inductive le_t (n : nat) : nat -> Type :=
+    | le_n : n <<= n
+    | le_S : forall m : nat, n <<= m -> n <<= S m
+  where "a <<= b" := (le_t a b).
+
+  Derive Signature NoConfusion for le_t.
+
+  Equations widen_fin {n n'} (H: n<<=n') (x : Fin.t n) : Fin.t n' :=
+    widen_fin (n:=0)   (n':=0)   _H          x := x;
+    widen_fin (n:=S a) (n':=S a) (le_n a)    x := x;
+    widen_fin (n:=0)   (n':=S a) _H  x := absurd_fin x; (* absurd *)
+    widen_fin (n:=S a) (n':=0)   H           x := _; (* absurd *)
+    widen_fin (n:=S a) (n':=S b) (le_S b H1) x with widen_fin H1 x => {
+        widen_fin (n:=S a) (n':=S b) (le_S b H2) _x y := FS y
+      }.
+  Next Obligation. inversion H. Qed.
+
+  (* A much nicer definition of [widen_fin] can be found here:
+     https://github.com/mattam82/Coq-Equations/blob/ded4baada11f9434333e53d9eb3c21ded33e67ad/examples/Fin.v#L58
+   *)
+
+  (*
+Inductive t : nat -> Set :=  F1 : forall n : nat, t (S n) | FS : forall n : nat, t n -> t (S n).
+   *)
+
+  Equations le_t_inj {n m} (H : S n <<= m) : n <<= m :=
+    le_t_inj (n:=n')         le_n := le_S n' n' (le_n n');
+    le_t_inj (n:=n') (m:=?(S (S m'))) (le_S (S m') H') with le_t_inj H' => {
+        le_t_inj (n:=n') (m:=?(S (S m'))) (le_S (S m') H') H'' := le_S _ _ H''
+      }.
+
+  Equations to_action {x_dim'} (rl : rule_name_t (S x_dim')) {x_dim_max : nat} (H: S x_dim' <<= S x_dim_max)
+    : uaction (reg_t (S x_dim_max)) (ext_fn_t (S x_dim_max)) :=
+
+    (* case: single router *)
+    to_action (rule 0 (@F1 ?(0))) le_n :=
       routestartfn 0
-        (reg_ regno idx) (* travel *)
-        (reg_ regno (nat_to_fin (0 + nocsize) ((nocsize-1) + nocsize)) (* output *)
-        (ex_ interfacesize (nat_to_fin 0 (nocsize * 2))) (* external in *)
-        (ex_ interfacesize (nat_to_fin 1 (nocsize * 2))); (* external out *)
+        (router  0 F1 state)
+        (router  0 F1 downstream)
+        (ext_fun 0 F1 input)
+        (ext_fun 0 F1 output);
 
-  @to_action (S noc_size') _pf (rule noc_size' idx) (F1 nocsize') :=
-    routeendfn noc_size'
-      (reg_ regno (nat_to_fin (Nat.pred n_idx) _ ))
-      (reg_ regno (nat_to_fin  (Nat.add (Nat.pred n_idx) noc_size') _))
-      (ex_ interfacesize (nat_to_fin (Nat.mul n_idx 2) _ ))i
-      (ex_ interfacesize (nat_to_fin (S (Nat.mul n_idx 2)) _))
+    (* case: first router in the pipeline *)
+    to_action (rule 0 (@F1 ?(0))) (x_dim_max:=n) H :=
+      let f1 := widen_fin H (@F1 0) in
+      routestartfn 0
+        (router  n f1 state)
+        (router  n f1 downstream)
+        (ext_fun n f1 input)
+        (ext_fun n f1 output);
 
-  @to_action (S noc_size) _pf (rule noc_size' idx) (F1 (S n)) :=
-      routecenterfn n_idx
-        (reg_ regno (nat_to_fin (Nat.pred n_idx) _ ))
-        (reg_ regno (nat_to_fin  n_idx _))
-        (reg_ regno (nat_to_fin  (Nat.add (Nat.pred n_idx) noc_size') _))
-        (ex_ interfacesize (nat_to_fin (Nat.mul n_idx 2) _ ))
-        (ex_ interfacesize (nat_to_fin (S (Nat.mul n_idx 2)) _))
-    @to_action (S noc_size) pf (rule noc_size' idx) (FS s) := to_action (S nocsize) pf (rule noc_size' s)
+    (* case : last router in the pipeline *)
+    to_action (rule (S c) (@F1 ?(S c))) (x_dim_max:=n) le_n :=
+      let f1  := @F1 (S c) in
+      let f1' := FS (@F1 c) in (* upstream *)
+      routeendfn (S c)
+        (router  (S c) f1  state)
+        (router  (S c) f1' downstream) (* upstream *)
+        (ext_fun (S c) f1  input)
+        (ext_fun (S c) f1  output);
 
+    (* case: center routers in the pipeline
+       (base case of the recursion)
+     *)
+    to_action (rule (S c) (@F1 ?(S c))) (x_dim_max:=n) (le_S n H) :=
+      let f1  := widen_fin (le_S _ _ H) (@F1 (S c)) in
+      let f1' := FS (widen_fin H (FS (@F1 c))) in (* upstream *)
+      routecenterfn n
+        (router  n f1  state)
+        (router  n f1' downstream) (* upstream *)
+        (router  n f1  downstream)
+        (ext_fun n f1  input)
+        (ext_fun n f1  output);
 
+    (* recursion *)
 
-      let n_idx := fin_to_nat idx in
-        if Nat.eqb n_idx 0 then
-        else if Nat.eqb n_idx noc_size' then
-        else
-.
-Next Obligation.
-  exfalso.
-  assert (bla : 1<nocsize). 1: { exact nocprop. }
-  rewrite <- pf in bla.
-  inversion bla.
-Qed.
-Next Obligation.
-  exfalso.
-  assert (bla : 1<nocsize). 1: { exact nocprop. }
-  rewrite <- pf in bla.
-  inversion bla.
-  inversion H0.
-Qed.
-Next Obligation. apply regno_gt_0. Qed.
-Next Obligation.
-  unfold regno.
-  rewrite <- _pf.
-  simpl.
-  rewrite <- Nat.succ_lt_mono.
-  rewrite -> plus_n_Sm.
-  apply Nat.lt_lt_add_l.
-  lia.
-Qed.
-Next Obligation. unfold interfacesize; lia. Qed.
-Next Obligation. unfold interfacesize; lia. Qed.
-Next Obligation.
-  unfold regno.
-  destruct nocsize.
-  - inversion _pf.
-  - inversion _pf.
-    subst. clear _pf.
-    induction idx eqn:E.
-    * unfold fin_to_nat; simpl; lia.
-    * specialize (IHt t eq_refl).
-      unfold fin_to_nat; fold (fin_to_nat t).
-      Search Nat.pred.
-  revert idx.
-  rewrite <- _pf.
-  intro idx.
-  dependent induction idx.
-  + unfold fin_to_nat.
-    simpl.
-    lia.
-  + unfold fin_to_nat.
-    simpl.
-    fold fin_to_nat.
-  dependent destruction idx.
-  - clear.
-  rewrite <- _pf in idx.
-  revert _pf.
-  destruct idx eqn:H.
-Obligations.
- 
-                            - apply regno_gt_0.
- - unfold regno. simpl.
-Qed.
-apply regno_gt_0.
-Next Obligation.
+    (* case: the fin space of the rule is smaller than the desired one *)
+    to_action (rule (S c) (FS c')) (x_dim_max:=n) (@le_S ?(S c) n H) :=
+      to_action (rule c c') (le_S _ n (le_t_inj H));
 
-Search nocsize.
-Check le_plus_trans.
-apply le_plus_l, nocprop.
-Search plus.
-apply nocprop.
-omega.
-Check le_S.
-Check le_n.  
-replace (nocsize + (nocsize - 1)) with (2 * nocsize - 1).
-apply Nat.lt_le_incl.
-
-Search nat. 
-Check Nat.lt.
-Check Nat.lt_le_incl.
-Check Nat.lt_alt.
-
-apply Nat.lt_le_incl.
+    (* case: the types of the fin space match up  *)
+    to_action (rule (S c) (FS c')) (x_dim_max:=?(S c)) H :=
+      to_action (rule c c') (le_t_inj H).
 
 
-
-
-
-
-Definition R ( reg : reg_t regno ) :=
-  match reg with
-  |  _ => bits_t (struct_sz basic_flit)
-  end.
-  
-Definition r (reg : reg_t regno) : R reg :=
-  match reg with
-  |  _ => Bits.zero
-  end.
-
-Definition Sigma' (fn: ext_fn_t interfacesize) : ExternalSignature :=
-  match fn with
-  | _ => {$ bits_t sz ~> bits_t sz $}
-  end.
-
-End NOCSetup.
-  (* Check tc_rules. *)
-(* 
-  Definition rules :=
-  tc_rules R Sigma'  to_action. *)
-
-(* Equations to_action' (nocsize:nat) (H: 1<=nocsize) (rl : rule_name_t nocsize) : uaction (reg_t regno) (ext_fn_t interfacesize) := 
-  (* to_action 0 H _ := { }; *)
-   to_action 1 (le_S n H1) _ with H1 := {} ; 
-   let idx := nat_to_fin nocsize 
-
-  to_action' (S nocsize') H (rule_ nocsize Fin.F1) :=
-    routestartfn 0 
-                (reg_ regno (nat_to_fin 0 _)) 
-                (reg_ regno (nat_to_fin nocsize' _)) 
-                (ex_ interfacesize (nat_to_fin 0 _)) 
-                (ex_ interfacesize (nat_to_fin 1 _));
-
-  to_action' (S nocsize') H (rule_ (S nocsize) n)  with n == (nat_to_fin nocsize') :=
-    | := routerend ...
-    | nocsize H (rule_ nocsize idx) :=
-        let n_idx := fin_to_nat idx in
-        routecenterfn n_idx 
-                (reg_ regno (nat_to_fin (Nat.pred n_idx) _ ))
-                (reg_ regno (nat_to_fin  n_idx _))
-                (reg_ regno (nat_to_fin  (Nat.add (Nat.pred n_idx) nocsize) _))
-                (ex_ interfacesize (nat_to_fin (Nat.mul n_idx 2) _ )) 
-                (ex_ interfacesize (nat_to_fin (S (Nat.mul n_idx 2)) _)).
-(* to_action nocsize H (rule_ nocsize n) := routecenterfn n (reg_ n) (reg_ (Nat.add nocsize n) ex_ 2n ex_ 2n+1) *)
-
-Equations to_action (nocsize:nat) (H: 2<=nocsize) (rl : rule_name_t nocsize) : uaction (reg_t regno) (ext_fn_t interfacesize) := 
-(* to_action 0 H _ := { }; *)
-  to_action 1 (le_S n H1) _ with H1 := {} ; 
-  to_action nocsize H _  := to_action' nocsize _ _;
-
-
-  to_action _ H r with r := 
-to_action' (Nat.sub nocsize 1) H rl.
-
-
-Definition to_action rl :=
-match rl with
-| router_ idx => let idx_nat := index_to_nat idx in
-  if Nat.eqb idx_nat 0 then (routestartfn 0 (reg 0)) 
-  else if Nat.eqb idx_nat regno then (routeendfn regno (reg (Nat.sub regno 1))) 
-  else (routecenterfn idx_nat (reg (Nat.sub idx_nat 1)) (reg idx_nat))  
-end.
- *)
-
- 
-(* Fixpoint nat_to_fin {n : nat} (m : nat) : option (Fin.t n) :=
-  match n return option (Fin.t n) with
-  | 0 => None (* No valid index if the bound is 0 *)
-  | S n' => match m with
-            | 0 => Some Fin.F1 (* The 0th index corresponds to Fin.F1 *)
-            | S m' => match nat_to_fin m' with
-                      | Some fin' => Some (Fin.FS fin') (* Successor index *)
-                      | None => None
-                      end
-            end
-  end.
-
-Compute @nat_to_fin 4 2.
-
-Inductive reg_t (num : nat) : Type :=
-  | reg_ : Fin.t num -> reg_t num.
-
-Inductive rule_name_t (num : nat) : Type :=
-  | rule_ : Fin.t num -> rule_name_t num.
-
-Inductive ext_fn_t (num : nat) : Type :=
-  | ext_ : Fin.t num -> ext_fn_t num.
-
-
-(*How is num correctly determined*)
-Definition reg_fn (num : nat) (n : nat) : option (reg_t num) :=  
-    match Fin.of_nat n num with
-    | inleft fin_idx => Some (reg_ num fin_idx)  (* Valid index, return register *)
-    | inright _ => None  (* Index out of bounds, return None *)
-    end.
-
-Definition rule_fn (num : nat) (n : nat) : option (rule_name_t num) :=
-    match Fin.of_nat n num with
-    | inleft fin_idx => Some (rule_ num fin_idx)  (* Valid index, return register *)
-    | inright _ => None  (* Index out of bounds, return None *)
-    end.
-
-Definition e_fn (num : nat) (n : nat) : option (ext_fn_t num) :=
-    match Fin.of_nat n num with
-    | inleft fin_idx => Some (ext_ num fin_idx)  (* Valid index, return register *)
-    | inright _ => None  (* Index out of bounds, return None *)
-    end.
-
-Search Fin.t. 
-Compute rule_ 2 (Fin.FS Fin.F1).
-Check rule_fn nocsize 0.
-(* Axiom rego_ge_1 : regno >= 1. (*
-  unfold regno.
-  induction nocsize eqn:H.
-  - set (H1 := nocprop).
-    rewrite H in H1.
-    unfold ">"%nat in H1.
-    apply Nat.nlt_succ_diag_l in H1.
-    contradiction.
-  - apply IHn. *)
-Definition reg_of_nat (n:nat) :reg_t.
-  set (a := index_of_nat regno n).
-  destruct a eqn:H.
-  - exact (reg_ i).
-  - unfold a in H.
-    destruct regno eqn:H1.
-    + admit.
-    + simpl in H.
-    unfold index_of_nat in H.
-    Admitted.
-
-Print index_of_nat.
-Definition reg_of_nat n :=
-  reg_ (match index_of_nat regno n with
-        | Some n => n
-        | None => thisone
-        end). *)
-
- (* Definition router n :=
-  router_ (match index_of_nat nocsize n with
-        | Some n => n
-        | None => thisone
-        end).   *)
- 
-(* Compute index 3.
-Compute index_of_nat nocsize 1.
-
-
-Fixpoint list_seq_index_anotherone {N : nat} (l : list (index N)) : list (index (S N)) :=
-  match l with
-  | nil => nil
-  | cons el l' => cons (anotherone el) (list_seq_index_anotherone l')
-  end.
-
-(* Constucting an ascending list of all possible indecies N *)
-Fixpoint list_seq_index (N : nat) : list (index N) :=
-  match N with
-  | O => nil
-  | S N' => cons (thisone) (list_seq_index_anotherone (list_seq_index N'))
-  end. 
-  
-Fixpoint get_nth_item_fin {A : Type} (l : list A) (n : Fin.t regno) : A :=
-  match l with
-  | [] => match n with end (* This case is impossible due to the dependent type *)
-  | x :: xs =>
-    match n with
-    | Fin.F1 => x
-    | Fin.FS n' => get_nth_item_fin xs n'
-    end
-  end. *)
-
-Module MyRegs <: Registers.
-Definition reg_t:=reg_t regno.
-Definition ext_fn_t:= ext_fn_t regno.
-End MyRegs.
-
-Module Routerfns:= Router(MyRegs)(MyTypes).        
-Import Routerfns.
-
-Check rule_fn.
-
-Definition to_action (rl: rule_name_t nocsize) := 
-match rl with
-| (rule_fn nocsize 0) => routestartfn 0 reg_fn regno 0 reg_fn regno 1 extfn interfacesize 0 extfn interfacesize 1
-| rule_ => routecenterfn 1 r1 r2 r5 extfn_3 extfn_4
-| rule_ => routecenterfn 2 r2 r3 r6 extfn_5 extfn_6
-| rule_ => routeendfn 3 r3 r7 extfn_7 extfn_8
-end.
-
-
-Equations to_action
- (rl : rule_name_t nocsize) : uaction (reg_t regno) (ext_fn_t interfacesize) := 
-to_action (rule_ nocsize) :=
-  let idx_nat := index_to_nat idx in
-  if Nat.eqb idx_nat 0 then
-    routestartfn 0 (reg_  indices 1)
-  else if Nat.eqb idx_nat regno then
-    let idx' := index_of_nat (Nat.sub idx_nat - 1) in
-    routeendfn regno (reg_ idx')
-  else
-    let idx' := index_of_nat (Nat.sub idx_nat - 1) in
-    routecenterfn idx_nat (reg_ idx') (reg_ idx).
-
- *)
-
-
-(* Compute Fin.of_nat_lt example_fin_auto.
-Compute @nat_to_fin 7 1 _.
-Check nat_to_fin.
-Compute Fin.of_nat_lt example_fin_auto.  
-Compute fin_to_nat (Fin.FS Fin.F1). *)
-
-(* Equations get_rule {nocsize:nat} (H: 1<=nocsize) (idx:Fin.t nocsize) : rule_name_t nocsize :=
-  (* get_rule 0   -> dicharged by equations *)
-  @get_rule (S n) _ idx := rule_ (S n) idx.
-
-Definition idx_zero (n:nat) : Fin.t (S n) := Fin.F1.
-Definition idx_one (n:nat) : Fin.t (S (S n)) := Fin.FS (idx_zero n).
-
-Definition lower_bound : Fin.t 4 := Fin.FS (Fin.FS (Fin.FS Fin.F1)).
-Print lower_bound.
-Print vect_nil.
-Print Fin.t.
-Inductive vec (T:Type) : nat -> Type :=
-  | vec_nil : vec T 0
-  | vec_append : forall n, T -> vec T n -> vec T (S n).
-
-Inductive myfin : nat -> Type :=
-  | myf1 : forall n, myfin (S n)
-  | myfs : forall n, myfin n -> myfin (S n).
-
-Check Fin.F1.
-
-Definition t_2 : Fin.t 3 :=  (Fin.FS (Fin.FS Fin.F1)).
-Equations idx' {n:nat} (i:Fin.t n) (ub:nat) :Fin.t n :=
-let 
-  idx' i'  0    := i';
-  idx' i' (S n) := idx' (Fin.FS i') n. 
-
-Equations idx (i:nat) (upper_bound:nat) (H: i<upper_bound)(H2: upper_bound>0) : Fin.t (S upper_bound) :=
-  idx 0 ub _ _ := @Fin.F1 ub;
-  idx (S n)
-
-Equations idx (i:nat) (sz:nat) (H: i<sz)(H2: sz>0)  : Fin.t sz :=
-  idx 0 _ _ _ := Fin.F1;
-  idx (S n) sz _ _ := @Fin.FS (S n) (idx n sz _ _ ).
-
-Equations rule_1 (nocsize:nat) (H: 1<=nocsize) (idx:Fin.t n) :rule_name_t nocsize:=
-  (* rule_1 0   *)
-  rule_1 (S 0) (le_S n H1) _ with H1 := {};
-  rule_1 (S (S n)) := rule_ nocsize (Fin.FS (Fin.FS (Fin.F1 n)). *)
+End Actions.
